---
title: Worksheet 16
subtitle: PH651, Fall 2021
author: Thomas Knudson
papersize: a4
geometry: margin=2cm
header-includes: |
    \usepackage{fancyhdr}
    \pagestyle{fancy}
    \fancyhead[RO,RE]{PH 651, Fall 2021}
    \fancyhead[CO,CE]{WS 16}
    \fancyhead[LO,LE]{Knudson}
---

\newcommand{\bra}[1]{{\left\langle#1\right|}}
\newcommand{\ket}[1]{{\left|#1\right\rangle}}

> Derive the action of the creation operator, $a^\dagger$ on an arbitrary eigenstate of the number operator $N$. $a^\dagger \ket{n} =\ ?$

Consider instead the result of acting the number operator on the quantity of $a^\dagger\ket{n}$: $Na^\dagger\ket{n}$. Since we're trying to determine the result of acting $a^\dagger$ on these kets, let's reorder the operators: we already know what $N$ acting on its eigenkets produces. To do this, let's work through the commutator of $N$ and $a^\dagger$:

$$\begin{aligned}
[N, a^\dagger] &= [a^\dagger a, a^\dagger]\\
&=a^\dagger [a, a^\dagger] + [a^\dagger, a^\dagger] a \\
&= a^\dagger (1) + (0) a \\
&= a^\dagger \\
Na^\dagger - a^\dagger N &= a^\dagger
\end{aligned}$$

Rearranging the last line, we see that $a^\dagger N + a^\dagger$ can be substituted in for $Na^\dagger$:

$$\begin{aligned}
Na^\dagger\ket{n} &= (a^\dagger N + a^\dagger)\ket{n}\\
&= a^\dagger N\ket{n} + a^\dagger\ket{n}\\
&= a^\dagger(n+1)\ket{n} \\
&= (n+1) a^\dagger\ket{n}
\end{aligned}$$

Now if we do a clever rename, as the result of an operator acting on a ket is a ket, we see:

$$
(a^\dagger\ket{n}) = \ket{?} \quad \Rightarrow \quad N\ket{?} = (n+1) \ket{?}
$$

However, we know that from the definition of $N$'s action on $\ket{n}$ what $\ket{?}$ must be to obtain the eigenvalue of $n+1$: $\ket{n+1}$. Therefore, we know, up to a scalar, the result of acting $a^\dagger$ on $\ket{n}$. To find the constant, we can simply evaluate the norm square of this statement:

$$\begin{aligned}
a^\dagger\ket{n} = c\ket{n+1} \Rightarrow \qquad\quad {\lvert a^\dagger\ket{n} \rvert}^2 &= {\lvert c\ket{n+1} \rvert}^2 \\
\bra{n}a a^\dagger\ket{n} &= {\lvert c \rvert}^2 \\
\bra{n}(1+a^\dagger a)\ket{n} &= {\lvert c \rvert}^2 \\
1+n &= {\lvert c \rvert}^2\\
c &= \sqrt{n+1}
\end{aligned}$$

Where we used the comutator of $[a, a^\dagger]=aa^\dagger - a^\dagger a = 1$ to substitute in an easier version.

$$a^\dagger \ket{n} = \sqrt{n+1} \ket{n+1}$$



