---
title: 1C
subtitle: MTH 420, S2022
author: Thomas Knudson
date: Monday, April 04, 2022
papersize: a4
geometry: margin=2cm
header-includes: |
    \usepackage{pgfplots}
    \usepackage{hyperref}
    \usepackage{tikz,tikz-3dplot} 
    \usepackage{tkz-euclide}
    \usepackage{fancyhdr}
    \usepackage{float}
    \usepackage{subcaption}
    \pagestyle{fancy}
    \fancyhead[RO,RE]{MTH 420, S2022}
    \fancyhead[CO,CE]{1C}
    \fancyhead[LO,LE]{Knudson}
---

## 1.3.8

> If each diagonal entry $a_{ii}$ is larger than the sum of the absolute values $|a_{ij}|$ along the rest of its row, then the symmetric matrix $A$ is positive definite. How large would $c$ have to be in \begin{equation} A = \begin{pmatrix} c & 1 & 1 \\ 1 & c & 1 \\ 1 & 1 & c \end{pmatrix} \end{equation} for this statement to apply? How large does $c$ actually have to be to assure that $A$ is positive definite? Note that \begin{equation}\label{eqn:quadFormProb1} x^T A x = (x_1 + x_2 + x_3)^2 + (c-1)({x_1}^2 + {x_2}^2 + {x_3}^2), \end{equation} when is this positive?

For the corollary given in the problem statement to be satisfied, we find that $c>2$. To determine how large $c$ actually has to be, we can examine the condition for positive eigenvalues of $A$. From the symmetric representation of $A$ in $L D L^T$, $D$ will be the diagonal matrix containing the eigenvalues of $A$, and all $d_i$ must be positive for $A$ to be a symmetric positive definite matrix.

We begin by setting up the eigenvalue equation, $\det{A-\lambda I}$, but with changing the constraint from equality with $0$ to greater than $0$, such that the determinant of $D$ will also be greater than $0$.

\begin{equation}
\begin{aligned}
\det{A-\lambda I} = \begin{vmatrix} c-\lambda & 1 & 1 \\ 1 & c-\lambda & 1 \\ 1 & 1 & c-\lambda \end{vmatrix} &> 0 \\
(c-\lambda)\bigg((c-\lambda)^2 -1\bigg) - ((c-\lambda) - 1) + (1 - (c-\lambda)) &> 0 \\
(c-\lambda)^3 - (c-\lambda) - (c-\lambda) + 1 + 1 - (c-\lambda) &> 0 \\
(c-\lambda)(c^2 - 2\lambda c + \lambda^2) - 3(c-\lambda) + 2 &> 0 \\
\underbrace{c^3 - 2\lambda c^2 + \lambda^2 c}_{c(c^2 - 2\lambda c + \lambda^2)} - \underbrace{\lambda c^2 + 2\lambda^2 c - \lambda^3}_{-\lambda(c^2 - 2\lambda c + \lambda^2)} - 3c + 3\lambda + 2 &> 0 \\
c^3 - 3c - \lambda^3  - 3 \lambda + 2 &> 0 \\
c^3 - 3c + 2 &> \lambda + 3\lambda
\end{aligned}
\end{equation}

Plotting this characteristic polynomial, we can see the two intervals that provide positive solutions are for $c\in(-2,1)$ and $c\in(1,\infty)$. Applying the condition that $c>0$ for $A$ to be positive definite, we can restrict the first interval to $c\in(0,1)$; however, this interval provides solutions that are incompatible with the problem statement's corollary. To further this conclusion, we can examine the quadratic form given with Equation \ref{eqn:quadFormProb1}, and note that for values of $c<1$, the second term becomes negative, which does not guarantee that the function $f=x^T A x$ is greater than $0$ (for $x\neq 0$) as required by page 18's definition for $A$ to be positive definite. As a result, the corollary will ensure that $A$ is positive definite with the finding that $c$ must be greater than $2$, but overlooks the valid interval of possible values for $c\in(1,2)$.

Therefore, $A$ will be positive definite as long as $c>1$.

\pagebreak

## 1.3.15

> Find the $LDL^T$ factorization, and the Cholesky's $\bar{L}\bar{L}^T$ factorization with $\bar{L} = LD^{1/2}$, for the matrix \begin{equation}A = \begin{pmatrix} 4 & 12 \\ 12 & 45 \end{pmatrix}. \end{equation} What is the connection to $x^T A x = (2x_1 + 6x_2)^2 + (3x_2)^2$?

We can find both factorizations simultaneously by noting that $A = L D L^T = \bar{L}\bar{L}^T$, which gives the following symbolic representation:

\begin{equation}
\begin{aligned}
\begin{pmatrix} a_{11} & a_{12} \\ a_{21} & a_{22} \end{pmatrix} &= \begin{pmatrix} \ell_{11} & 0 \\ \ell_{21} & \ell_{22} \end{pmatrix} \begin{pmatrix} d_{11} &0 \\ 0 & d_{22} \end{pmatrix} \begin{pmatrix} \ell_{11} & \ell_{12} \\ 0 & \ell_{22} \end{pmatrix} &&= \begin{pmatrix} \bar{\ell}_{11} & 0 \\ \bar{\ell}_{21} & \bar{\ell}_{22} \end{pmatrix} \begin{pmatrix} \bar{\ell}_{11} & \bar{\ell}_{12} \\ 0 & \bar{\ell}_{22} \end{pmatrix}\\
\begin{pmatrix} a_{11} & a_{12} \\ a_{12} & a_{22} \end{pmatrix} &= \begin{pmatrix} \ell_{11} & 0 \\ \ell_{21} & \ell_{22} \end{pmatrix} \begin{pmatrix} d_{11} &0 \\ 0 & d_{22} \end{pmatrix} \begin{pmatrix} \ell_{11} & \ell_{21} \\ 0 & \ell_{22} \end{pmatrix} &&= \begin{pmatrix} \bar{\ell}_{11} & 0 \\ \bar{\ell}_{21} & \bar{\ell}_{22} \end{pmatrix} \begin{pmatrix} \bar{\ell}_{11} & \bar{\ell}_{21} \\ 0 & \bar{\ell}_{22} \end{pmatrix},
\end{aligned}
\end{equation}

where we have used the symmetry to simplify $a_{12}=a_{21}$,  $\ell_{12}=\ell_{21}$, and $\bar{\ell}_{12}=\bar{\ell}_{21}$. From this, we obtain the system of equations

\begin{equation}\label{eqn:origSys}
\begin{aligned}
a_{11} &= \ell_{11}d_{11}\ell_{11} &&= {\bar{\ell}_{11}}^2\\
a_{12} &= \ell_{11}d_{11}\ell_{21} &&= \bar{\ell}_{11}\bar{\ell}_{21} \\
a_{22} &= {\ell_{21}}d_{11}{\ell_{21}} + \ell_{22}d_{22}\ell_{22} &&= {\bar{\ell}_{21}}^2 + {\bar{\ell}_{22}}^2
\end{aligned},
\end{equation}

and begin simplifying by performing one row operation on $A$ to obtain an upper triangular matrix, which provides the necessary value for $\ell_{21}$:

\begin{equation}
\begin{aligned}
A_2 &= A_2 - 3 A_1 \\
A^\prime &= \begin{pmatrix} 4 & 12 \\ 0 & 45 \end{pmatrix}
\end{aligned}.
\end{equation}

Substituting in $3$ for $\ell_{21}$ alongside all the values of $a_{ij}$, we rewrite the system of equations \ref{eqn:origSys} as:

\begin{align}
4 &= \ell_{11}d_{11}\ell_{11}\\
12 &= 3\ell_{11}d_{11}\\
45 &= (3)^2 d_{11} + \ell_{22}d_{22}\ell_{22}
\end{align}

Then by solving Equations 8 and 9 for $d_{11}$ and comparing, we find that $\ell_{11}$ must be $1$ for both equations to be satisfied.

\begin{equation*}
\frac{4}{{\ell_{11}}^2} = d_{11} = \frac{4}{\ell_{11}} \Rightarrow d_{11} = 4
\end{equation*}

By dividing Equation 6 by $\ell_{11}$, we can substitute this result into Equation 7 and find that $\ell_{21}$ is scalar multiple of $\ell_{11}$. Summarizing our results so far, we revisit the matrix representation of $A = L D L^T = \bar{L}\bar{L}^T$ and our final remaining equation from the original system:

\begin{equation}
\begin{aligned}
\begin{pmatrix} 4 & 12\\ 12 & 45 \end{pmatrix} &= \begin{pmatrix} 1 & 0 \\ 3 & \ell_{22} \end{pmatrix} \begin{pmatrix} 4 &0 \\ 0 & d_{22} \end{pmatrix} \begin{pmatrix} 1 & 3 \\ 0 & \ell_{22} \end{pmatrix} &&= \begin{pmatrix} \pm 2 & 0 \\ \bar{\ell}_{21} & \bar{\ell}_{22} \end{pmatrix} \begin{pmatrix} \pm 2 & \bar{\ell}_{21} \\ 0 & \bar{\ell}_{22} \end{pmatrix},
\end{aligned}
\end{equation}

\begin{equation}
45 = 4(3)^2 + {\ell_{22}}^2 d_{22} = {\bar{\ell}_{21}}^2 + {\bar{\ell}_{22}}^2
\end{equation}

Noting that the product of $\ell d \ell^T$ that corresponds to $\bar{\ell}_{21}$ is given by $\ell_{11}d_{11}\ell_{21}$, we obtain $\bar{\ell}_{21}$:

\begin{equation}
\begin{aligned}
\bar{\ell}_{21} &= \sqrt{d_{11}}\ell_{21} \\
&= \pm 6
\end{aligned}.
\end{equation}

We take the positive value of $6$ for $\bar{\ell}_{21}$, such that $\bar{L}^T = (\bar{L})^T$. Finally, we can obtain $d_{22}$ by computing the $\det{A}$ and recalling that the determinant is equal to the product of the eigenvalues. Since $\det{A}=36$ and $d_{11}=4$, $d_{22}$ must be $9$. Substituting these results into Equation 10, we find that ${\ell_{22}}^2$ must also be $1$.

\begin{align*}
45 &= 36 + 9 {\ell_{22}}^2\\
1 &= {\ell_{22}}^2
\end{align*}

Summarizing our findings, like in Equation 11, we have the following:

\begin{equation*}
\begin{aligned}
\begin{pmatrix} 4 & 12\\ 12 & 45 \end{pmatrix} &= \begin{pmatrix} 1 & 0 \\ 3 & \pm 1 \end{pmatrix} \begin{pmatrix} 4 & 0 \\ 0 & 9 \end{pmatrix} \begin{pmatrix} 1 & 3 \\ 0 & \pm 1 \end{pmatrix} &&= \begin{pmatrix} \pm 2 & 0 \\ 6 & (\pm 3)(\pm 1) \end{pmatrix} \begin{pmatrix} \pm 2 & 6 \\ 0 & (\pm 3)(\pm 1) \end{pmatrix}.
\end{aligned}
\end{equation*}

Through simple trial and error (there are only 2 solutions to check), we conclude that $\ell_{22}$ must be positive for $L D L^T$ to produce $A$, which similarly requires $\bar{\ell}_{11}$ and $\bar{\ell}_22$ to be positive. The final factorizations of $A$ are then given by:

\begin{equation}
\begin{aligned}
\begin{pmatrix} 4 & 12\\ 12 & 45 \end{pmatrix} &= \begin{pmatrix} 1 & 0 \\ 3 & 1 \end{pmatrix} \begin{pmatrix} 4 & 0 \\ 0 & 9 \end{pmatrix} \begin{pmatrix} 1 & 3 \\ 0 & 1 \end{pmatrix} &&= \begin{pmatrix} 2 & 0 \\ 6 & 3 \end{pmatrix} \begin{pmatrix} 2 & 6 \\ 0 & 3 \end{pmatrix},
\end{aligned}
\end{equation}

and the connection to $x^T A x = (2x_1 + 6x_2)^2 + (3x_2)^2$ is made evident that the scalars for each $x_i$ correspond to the entries in the Cholesky factorization. This is trivial to verify through carrying out the requisite matrix multiplication:

\begin{equation*}
\begin{aligned}
\begin{pmatrix} x_1 & x_2 \end{pmatrix} \begin{pmatrix} a_{11} & a_{12} \\ a_{12} & a_{22} \end{pmatrix} \begin{pmatrix} x_1 \\ x_2 \end{pmatrix} &= \begin{pmatrix} 4x_1 + 12x_2 & 12x_1 + 45x_2 \end{pmatrix}\begin{pmatrix} x_1 \\ x_2 \end{pmatrix} \\
&= {x_1}(a_{11}x_1 + a_{12}x_2) + {x_2}(a_{12}x_1 + a_{22}x_2) \\
&= a_{11}{x_1}^2 + 2 a_{12} x_1 x_2 + a_{22}{x_2}^2 \\
&= {\bar{\ell}_{11}}^2 {x_1}^2 + 2 {\bar{\ell}_{12}} x_1 x_2 + ({\bar{\ell}_{21}}^2 + {\bar{\ell}_{22}}^2){x_2}^2 \\
&= (\bar{\ell}_{11}x_1 + \bar{\ell}_{12}x_2)^2 + (\bar{\ell}_{22}x_2)^2 \\
&= (2x_1 + 6x_2)^2 + (3x_2)^2
\end{aligned}
\end{equation*}
