$$\gdef\wrap[2]{\left( #1 \right)_{ #2 }}$$
$$\gdef\pder[2]{\frac{\partial #1}{\partial #2}}$$
$$\gdef\pdersq[2]{\frac{\partial^2 #1}{\partial^2 #2}}$$
$$\gdef\mpder[3]{\frac{\partial^2 #1}{\partial #2\partial #3}}$$

# PH 541: Statistical Mechanics

Course Content Outline:
- Review of macroscopic thermodynamics
- Foundations of statistical Mechanics
- Canonical ensemble
- Ideal Gas
- Black body radiation
- Grand canonical ensemble
- Ideal Fermi and Bose gases

----

## Week 1

### Day 1
First 2-3 Weeks:
 - Review Thermal Physics (Macroscopic)

Week 4-10:
 - Statistical Physics
 - Microscopic thermodynamics

#### Macroscopic Thermodynamics
There are four laws of Thermodynamics: (page 122-123)
1. Thermal Equilibrium
2. $dE = -đW + đQ$
3. Principle of the Increase of Entropy
4. Minimal Entropy

##### The Zeroth Law
?> if two thermodynamic systems are each in thermal equilibrium with a third system, then they are in thermal equilibrium with each other.

##### The First Law

- Conservation of Energy
- $E$ is the internal energy of the system
  - $dE$ is a change of the internal energy ([exact](/maths/Differentials.md) & total differential)
  - a function of the state of the system
    - E.g., for a gas in a bottle, the state of the system is described by number of molecules, volume, and temperature.
- $W$ is work
  - $\bar{d}W$ is an [inexact](/maths/Differentials.md) differential
  - The work you have to do is not determined by the state of the system; but by the process.
  - Not a state function
- $Q$ is heat transfer
  - $\text{đ}Q$ is the heat absorbed by the system.

Reversible
- The first law becomes: $dE=đQ-pdV$
  - an Isolated system receives no heat energy, so $dE=-pdV$
  - Otherwise, the system absorbs heat through a quasistatic process:
    - $đQ=TdS$


##### The Second Law

Describes the direction of natural processes.
  - E.g., heat cannot (naturally) transfer from a colder body to a hotter body

We can quantify the macroscopic state of a system using [Entropy](/physics/Entropy.md).
For an isolated system:
$$\Delta S_{system} \geq 0$$

If the system is not isolated and undergoes a quasistatic infinitesimal process in which it absorbs heat $dQ$, then:
$$dS=\frac{đQ}{T} \Leftrightarrow TdS=đQ$$

----

### Day 2

Review of last class's concepts:
- $đQ=dE+đW$
  - We can decompose the heat into kinetic and potential energy.
- Definition of change of entropy:
  - if the system is isolated and undergoes an infinitesimal quasistatic process
    - $dS=\frac{đQ}{T}$
  - if the system is isolated and we go from one macroscopic state to another:
    - $\Delta S \geq 0$
    - **Thermally Isolated**, $\Delta S$ cannot be less than $0$
  - called the: Principle of the Increase of Entropy
  - Clausius's Statement:
    - "Heat cannot, by itself, pass from a colder to a hotter body"
$$\begin{aligned}
\Delta S &= \frac{-đQ}{T_A}+\frac{đQ}{T_B} \\
&= đQ\left(\frac{1}{T_B}-\frac{1}{T_A}\right) < 0
\end{aligned}$$
  - Kelvin's Statement:
    - "A process whose **only** effect is the **complete** conversion of Heat (energy) into Work cannot occur."
      - $đQ\rightarrow đW$
      - $dS = \frac{-đQ}{T} < 0$
    - This is why engines cannot have $100$ % efficiency

!> Statements in Thermodynamics must be precise. Lacking keywords can invalidate the entire statement.

##### The Third Law

The limiting property of entropy:

?> As the temperature of a system approaches absolute zero, all processes cease and the entropy of the system approaches a minimum value.  $T\rightarrow 0_+,\qquad S\rightarrow S_0 = 0$

We'll discuss this later in the course.

#### Review of Math in Thermodynamics

##### Rules of total derivatives

Consider two single variable functions: $f(x),\ g(x)$

###### Linearity
$$\frac{d}{dx}(f(x)+g(x))=\frac{d}{dx}f(x)+\frac{d}{dx}g(x)$$

###### Product rule
$$\frac{d}{dx}(f(x)\cdot g(x))=f(x)\frac{d}{dx}g(x)+g(x)\frac{d}{dx}f(x)$$
$$\frac{d}{dx}\left(\frac{f(x)}{g(x)}\right)=\left(f(x)\frac{d}{dx}g(x)-g(x)\frac{d}{dx}f(x)\right)\cdot\left(\frac{1}{g(x)^2}\right)$$

###### Chain rule
$$f(U(x))$$
$$\frac{df}{dx}=\frac{df}{du}\cdot\frac{du}{dx}$$

##### Rules for Partial derivatives

Let $E$ be the energy of the system.
$$E=E(T,V) = E(p, V) = E(p, T)$$

Any two thermodynamic variables are independent. However, if you look at three parameters together, you cannot change them independently of each other.

Consider the multivariable function $f(x,y)$:

$$\left(\frac{\partial f}{\partial x}\right)_y$$
- Describes the change of $f$ as the result of the change of $x$ while keeping $y$ fixed/constant

!> Always write the specific parameters that are held constant.

###### Clauriet's Theorem
$$\left(\frac{\partial}{\partial y}\right)_x \left(\frac{\partial f}{\partial x}\right)_y = \frac{\partial^2 f}{\partial x\partial y} = \frac{\partial^2 f}{\partial y\partial x} = \left(\frac{\partial}{\partial x}\right)_y \left(\frac{\partial f}{\partial y}\right)_x$$

We use this to derive [Maxwell's Relations].

###### Reciprocal Rule

$f(x,y)=0$

$$df=\left(\frac{\partial f}{\partial x}\right)_y dx + \left(\frac{\partial f}{\partial y}\right)_x dy$$
Consider $df=0$ because $f(x,y)=0$:
$$0=\left(\frac{\partial f}{\partial x}\right)_y dx + \left(\frac{\partial f}{\partial y}\right)_x dy$$
$$\left(\frac{\partial f}{\partial x}\right)_y dx = - \left(\frac{\partial f}{\partial y}\right)_x dy$$
$$\left(\frac{dx}{dy}\right) = - \frac{ \left(\frac{\partial f}{\partial y}\right)_x}{\left(\frac{\partial f}{\partial x}\right)_y}$$

We can rewrite: $f(x,y)=0$ as $x(f,y)$ or $y(f,x)$ which means the left-hand side should really be partial derivatives

$$\left(\frac{\partial x}{\partial y}\right)_f = - \frac{ \left(\frac{\partial f}{\partial y}\right)_x}{\left(\frac{\partial f}{\partial x}\right)_y}$$

Repeat the same process and we obtain the following:

$$\left(\frac{\partial y}{\partial x}\right)_f = - \frac{ \left(\frac{\partial f}{\partial x}\right)_y}{\left(\frac{\partial f}{\partial y}\right)_x}$$

Which shows us that they're inversely related to each other:

$$\left(\frac{\partial x}{\partial y}\right)_f = \frac{1}{\left(\frac{\partial x}{\partial y}\right)_f}$$

###### Cyclic Rule:

$f(x,y,z)=0$

$$\left(\frac{\partial x}{\partial y}\right)_z \left(\frac{\partial z}{\partial x}\right)_y \left(\frac{\partial y}{\partial z}\right)_x = -1$$

Proving this rule is the same as the Reciprocal Rule.
- $df(x,y,z)=0$
  - $df = \left(\frac{\partial f}{\partial x}\right)_{y,z} dx + \left(\frac{\partial f}{\partial y}\right)_{x,z} dy + \left(\frac{\partial f}{\partial z}\right)_{x,y} dz$
- treat $z$ constant
  - $df = 0 = dz$
  - $\left(\frac{\partial x}{\partial y}\right)_z = - \frac{\left(\frac{\partial f}{\partial y}\right)_{x,z}}{\left(\frac{\partial f}{\partial x}\right)_{y,z}}$
- treat $x$ constant
  - $df = 0 = dx$
  - $\left(\frac{\partial y}{\partial z}\right)_x = - \frac{\left(\frac{\partial f}{\partial z}\right)_{x,y}}{\left(\frac{\partial f}{\partial y}\right)_{x,z}}$
- treat $y$ constant
  - $df = 0 = dy$
  - $\left(\frac{\partial z}{\partial x}\right)_y = - \frac{\left(\frac{\partial f}{\partial x}\right)_{y,z}}{\left(\frac{\partial f}{\partial z}\right)_{x,y}}$

$$\left(\frac{\partial x}{\partial y}\right)_z \left(\frac{\partial z}{\partial x}\right)_y \left(\frac{\partial y}{\partial z}\right)_x = -1$$

----

### Day 3

We're going to use the math tools from the previous class to look at:
- Van der Waals gas
- Volumetric compressibility

Simple Application of Macroscopic Thermodynamics (page 152-200)

#### Van der Waals gas

$$p=\frac{nRT}{V-nb}-a\frac{n^2}{V^2}$$

- $V$ is the total volume
- $nb$ is a correct term to subtract the volume occupied by the molecules

##### Isothermal compressibility: $K_t$

$$K_t\equiv -\frac{1}{V}\left(\frac{\partial V}{\partial p}\right)_T$$

- normalized with respect to the volume

##### Isobaric Volumetric thermal expansion coefficient

$$\alpha \equiv \frac{1}{V}\left(\frac{\partial V}{\partial T}\right)_p$$


$$P=p(V,T)$$
$$P=p(V,T)=\frac{nRT}{V-nb}-a\frac{n^2}{V^2}$$

$$\left(\frac{\partial p}{\partial T}\right)_V = \frac{nR}{V-nb}$$
$$\left(\frac{\partial p}{\partial V}\right)_T = -\frac{nRT}{(V-nb)^2} + 2\frac{an^2}{V^3}$$

Using Reciprocal Rule:
$$K_t\equiv -\frac{1}{V}\left(\frac{\partial V}{\partial p}\right)_T = -\frac{1}{V}\frac{1}{\frac{nR}{V-nb}} = -\frac{1}{V}\frac{V-nb}{nr} $$

Using the Cyclic Rule:
$$\begin{aligned}
\alpha &= \frac{1}{V}\left(\frac{\partial V}{\partial T}\right)_p \\
&= \frac{1}{V} \left( -\left(\frac{\partial T}{\partial p}\right)_V \left(\frac{\partial p}{\partial V}\right)_T \right)^{-1} \\
&= -\frac{1}{V} \left( \left(\frac{V-nb}{nr}\right) \left(-\frac{nRT}{(V-nb)^2} + 2\frac{an^2}{V^3}\right) \right)^{-1}
\end{aligned}$$

#### Properties of Ideal Gas

Equation of State:
$$pV=nRT$$

For an ideal gas, we can take the following statement:
$E=E(T,V)$ and show that $E$ only depends on $T$: $E=E(T)$ which implies
$$\left(\frac{\partial E}{ \partial V}\right)_T \equiv 0$$

First, we take the total derivative:

$$\begin{aligned}
dE &= dE(T,V) \\
&=\left(\frac{\partial E}{ \partial T}\right)_V dT + \left(\frac{\partial E}{ \partial V}\right)_T dV
\end{aligned}$$

Then also consider the First Law of Thermo:

$$\begin{aligned}
TdS &= dE + pdV \\
dS &= \frac{1}{T}dE + \frac{p}{T}dV
\end{aligned}$$

Note that because we can write the differential of entropy as a total derivative, this tells us that $dS$ is an exact differential, which means we can write:
$$\begin{aligned}
S &= S(E,V) \\
 &= \left(\frac{\partial S}{\partial E}\right)_V dE + \left(\frac{\partial S}{\partial V}\right)_E dV
\end{aligned}$$

Because there is only one way to write the total derivative, we know the coefficients for the differntials are equal to the partial derivatives stated above:

$$\frac{1}{T} = \left(\frac{\partial S}{\partial E}\right)_V$$
- Which is the definition of temperature in macroscopic Thermodynamics

$$\frac{p}{T} = \left(\frac{\partial S}{\partial V}\right)_E$$
- Which is the definition of temperature without knowing Microscopic details

Also recall that with mixed partial derivatives, the order of operations doesn't matter (Clauriet's Theorem):

$$\frac{\partial ^2 S}{\partial V \partial E} = \frac{\partial ^2 S}{\partial E \partial V}$$

$$\begin{aligned}
\frac{\partial ^2 S}{\partial V \partial E} &= \left(\frac{\partial }{\partial V}\right)_E \left(\frac{\partial S}{\partial E}\right)_V \\
\frac{\partial ^2 S}{\partial E \partial V} &= \left(\frac{\partial }{\partial E}\right)_V \left(\frac{\partial s}{\partial V}\right)_E
\end{aligned}$$

---

$$\begin{aligned}
dS &= \frac{1}{T}dE + \frac{p}{T}dV \\
dE &= \left(\frac{\partial E}{ \partial T}\right)_V dT + \left(\frac{\partial E}{ \partial V}\right)_T dV \\
\\
dS &= \frac{1}{T}\left(\left(\frac{\partial E}{ \partial T}\right)_V dT + \left(\frac{\partial E}{ \partial V}\right)_T dV\right) + \frac{p}{T}dV \\
&= \frac{1}{T}\left(\frac{\partial E}{ \partial T}\right)_V dT + \left(\frac{1}{T}\left(\frac{\partial E}{ \partial V}\right)_T + \frac{p}{T}\right)dV \\
\\
dS &= \left(\frac{\partial S}{\partial T}\right)_V dT + \left(\frac{\partial S}{\partial V}\right)_T dV \\
\\
\\
\left(\frac{\partial S}{\partial T}\right)_V &= \frac{1}{T}\left(\frac{\partial E}{ \partial T}\right)_V \\
\left(\frac{\partial S}{\partial V}\right)_T &= \left(\frac{1}{T}\left(\frac{\partial E}{ \partial V}\right)_T + \frac{p}{T}\right)
\end{aligned}$$

Then:

$$\begin{aligned}
\left(\frac{\partial }{\partial V}\right)_T \left(\frac{\partial S}{\partial T}\right)_V &\equiv \left(\frac{\partial }{\partial T}\right)_V \left(\frac{\partial S}{\partial V}\right)_T \\
\frac{1}{T} \left(\frac{\partial^2 E}{\partial V\partial T}\right) &= \left(\frac{\partial}{\partial T}\right)_V \left[\frac{1}{T}\left(\frac{\partial E}{\partial V}\right)_T + \frac{p}{T}\right] \\
\frac{1}{T} \left(\frac{\partial^2 E}{\partial V\partial T}\right) &= \frac{1}{T} \left(\frac{\partial^2 E}{\partial V\partial T}\right) + \frac{1}{T^2} \left(\frac{\partial E}{\partial V}\right)_T \\
0 &= \frac{1}{T^2} \left(\frac{\partial E}{\partial V}\right)_T
\end{aligned}$$

---

## Week 2

### Day 2

#### SWBQ from last class:
Show that for an ideal gas that undergoes a adiabatic expansion or compression, the equation of state statisfies:

$$\begin{aligned}
pV^\gamma &= \text{constant} \\
&\text{where }\gamma = (1+\frac{R}{C_V})=\frac{C_p}{C_V}
\end{aligned}$$

Zap with d:

$$\begin{aligned}
d(pV) &= nRdT \\
pdV+Vdp &= nRdT
\end{aligned}$$

Use first law:
$$\begin{aligned}
\bar{d}Q &= dE+\bar{d}W \\
&dQ = 0 \text{ (adiabatic)} \\
&dE = nC_v dT \\
&\bar{d}W = pdV \\
0 &= nC_v dT + pdV \\
pdV &= - nC_v dT
\end{aligned}$$

Substitute and continue:

$$\begin{aligned}
pdV+Vdp &= -\frac{Rp}{C_v}dV \\
pdV+\frac{Rp}{C_v}dV &= -Vdp
\end{aligned}$$

#### Entropy of an ideal gas

Ideal gas is sometimes referred to as a "perfect gas" (gas molecules do not interact to have any potential energy; all energy comes from kinetic)

SWBQ

Consider $n_0$ moles of an ideal gas that occupies a volume $V_0$ and at the temperature $T_0$. Let $S_0$ be the molar entropy of the gas at this specific macroscopic state (macro state).

> Molar entropy is the entropy of one mole of this gas.

Calculate the entropy $S(T,V,n)$ of the gas at $T$ and $V$.
- start with first law
- solve for dS
- use $dE$ in terms of molar specific heat capcity
  - we can only do this substitution because we have an ideal gas
  - energy does not depend on internal volume
- use $pV=nRT$ to rewrite $p$ in terms of given variables
- integrate
  - approximate that $C_V(T)$ is constant over small change in $T$


$$\begin{aligned}
\int_{(T_0, V_0)}^{(T,V)}{dS} &= \int_{T_0}^{T}{nC_V(T)\frac{dT}{T}} + \int \\
Sn-S_0 n_0 &= n\left(\ln{\left(\frac{T}{T_0}\right)}^{C_V} + \ln{\left(\frac{V}{V_0}\right)}^R\right) \\
Sn &= n\left(\ln{\left(\frac{T}{T_0}\right)}^{C_V} + \ln{\left(\frac{V}{V_0}\right)}^R\right) + S_0 n_0 \\
S &= \left(\ln{\left(\frac{T}{T_0}\right)}^{C_V} + \ln{\left(\frac{V}{V_0}\right)}^R\right) + S_0\frac{n_0}{n} \\
S(T,V,n) &= n\left(C_V\ln{(T)}+R\ln{(V)}+S_0(T_0,V_0)\right)
\end{aligned}$$

### Day 3
Today:
- Investigate general relation for homogeneous substance
  - E.g., liquids, gases, solids
- Derive Maxwell's Relations
  - page 161 to page 170

## Maxwell's Relations

### Recap

Start with the First Law:

$$\begin{aligned}
\bar{d}Q &= dE + \bar{d}W
\end{aligned}$$

In the case the system undergoes a quasi-static process (at each step, the system can be considered at equilibrium)

$$\begin{aligned}
TdS &= dE + pdV \\
dS &= \frac{1}{T}dE + \frac{p}{T}dV
\end{aligned}$$

!> recall that if we can write a differential as a total differential, we can conclude: $S=S(E,V)$

$$dS = \left(\frac{\partial S}{\partial E}\right)_V dE + \left(\frac{\partial S}{\partial V}\right)_E dV$$

This tells us that the partial derivatives must be equal to the coefficients of the differentials in the statement above:

$$\begin{aligned}
\left(\frac{\partial S}{\partial E}\right)_V &= \frac{1}{T}\\
\left(\frac{\partial S}{\partial V}\right)_E &= \frac{p}{T}
\end{aligned}$$

### From there

- We can choose any 2 parameters as independent variables

#### E with S and V independent

So, let's try choosing $S$ and $V$ as our independent variables:

$$\begin{aligned}
TdS &= dE + pdV \\
dE &= TdS - pdV \\
\\
E &= E(S,V) \\
\\
dE &= \left(\frac{\partial E}{\partial S}\right)_V dS + \left(\frac{\partial E}{\partial V}\right)_S dV \\
\\
\left(\frac{\partial E}{\partial S}\right)_V &= T \\
\left(\frac{\partial E}{\partial V}\right)_S &= -p
\end{aligned}$$

Order of second partial derivative doesn't matter -> Clauriet's Theorem

$$\begin{aligned}
\left(\frac{\partial }{\partial V}\right)_S \left(\frac{\partial}{\partial S}\right)_V E &= \frac{\partial^2 E}{\partial V\partial S} \\
\frac{\partial^2 E}{\partial V\partial S} &= \frac{\partial^2 E}{\partial S\partial V}\\
\frac{\partial^2 E}{\partial S\partial V} &= \left(\frac{\partial }{\partial S}\right)_V \left(\frac{\partial}{\partial V}\right)_S E
\end{aligned}$$

We can use this to rewrite:

$$\begin{aligned}
\left(\frac{\partial }{\partial V}\right)_S T &= \left(\frac{\partial T}{\partial V}\right)_S \\
\left(\frac{\partial }{\partial S}\right)_V \left(-p\right) &= -\left(\frac{\partial p}{\partial S}\right)_V \\
\\
\left(\frac{\partial T}{\partial V}\right)_S &= -\left(\frac{\partial p}{\partial S}\right)_V
\end{aligned}$$

#### H with S and p independent

Start with First Law, be we want $dS$ and $dp$ (not $dV$)

$$\begin{aligned}
TdS &= dE + pdV \\
dE &= TdS - pdV - Vdp + Vdp\\
dE &= TdS - d(pV) + Vdp\\
dE + d(pV) &= TdS + Vdp\\
d(E+pV) &= TdS + Vdp\\
\\
H &= E + pV \equiv \text{ Enthalpy}\\
\\
dH &= TdS + Vdp\\
H &= H(S,p)\\
\\
dH &= \left(\frac{\partial H}{\partial S}\right)_p dS + \left(\frac{\partial H}{\partial p}\right)_S dp \\
\\
\left(\frac{\partial H}{\partial S}\right)_p &= T \\
\left(\frac{\partial H}{\partial p}\right)_S &= V
\end{aligned}$$

Order of second partial derivative doesn't matter -> Clauriet's Theorem

$$\begin{aligned}
\left(\frac{\partial }{\partial p}\right)_S \left(\frac{\partial}{\partial S}\right)_p H &= \frac{\partial^2 H}{\partial p\partial S} \\
\frac{\partial^2 H}{\partial p\partial S} &= \frac{\partial^2 H}{\partial S\partial p}\\
\frac{\partial^2 H}{\partial S\partial p} &= \left(\frac{\partial }{\partial S}\right)_p \left(\frac{\partial}{\partial p}\right)_S H
\end{aligned}$$

We can use this to rewrite:

$$\begin{aligned}
\left(\frac{\partial }{\partial p}\right)_S T &= \left(\frac{\partial T}{\partial p}\right)_S \\
\left(\frac{\partial }{\partial S}\right)_p V &= \left(\frac{\partial p}{\partial S}\right)_p \\
\\
\left(\frac{\partial T}{\partial p}\right)_S &= \left(\frac{\partial V}{\partial S}\right)_p
\end{aligned}$$

#### F with T and V independent

Start with First Law, be we want $dS$ and $dp$ (not $dV$)

$$\begin{aligned}
TdS &= dE + pdV \\
dE &= TdS - pdV + SdT + Vdp\\
dE &= TdS - d(pV) + Vdp\\
dE + d(pV) &= TdS + Vdp\\
d(E+pV) &= TdS + Vdp\\
\\
H &= E + pV \equiv \text{ Enthalpy}\\
\\
dH &= TdS + Vdp\\
H &= H(S,p)\\
\\
dH &= \left(\frac{\partial H}{\partial S}\right)_p dS + \left(\frac{\partial H}{\partial p}\right)_S dp \\
\\
\left(\frac{\partial H}{\partial S}\right)_p &= T \\
\left(\frac{\partial H}{\partial p}\right)_S &= V
\end{aligned}$$

Order of second partial derivative doesn't matter -> Clauriet's Theorem

$$\begin{aligned}
\left(\frac{\partial }{\partial p}\right)_S \left(\frac{\partial}{\partial S}\right)_p H &= \frac{\partial^2 H}{\partial p\partial S} \\
\frac{\partial^2 H}{\partial p\partial S} &= \frac{\partial^2 H}{\partial S\partial p}\\
\frac{\partial^2 H}{\partial S\partial p} &= \left(\frac{\partial }{\partial S}\right)_p \left(\frac{\partial}{\partial p}\right)_S H
\end{aligned}$$

We can use this to rewrite:

$$\begin{aligned}
\left(\frac{\partial }{\partial p}\right)_S T &= \left(\frac{\partial T}{\partial p}\right)_S \\
\left(\frac{\partial }{\partial S}\right)_p V &= \left(\frac{\partial p}{\partial S}\right)_p \\
\\
\left(\frac{\partial T}{\partial p}\right)_S &= \left(\frac{\partial V}{\partial S}\right)_p
\end{aligned}$$

### SWBQ

We've found the relations for:
- $S,p$
- $S,V$

What about:
- $T,V$?



\left(\frac{\partial }{\partial }\right)_

## Week 3

### Day 1

Won't be asked to derive the Maxwell Relations again, but we may want to use them to answer questions asked that either don't provide an easy or straightforward avenue.

Objectives:
 - Specific Heats
  - heat capacity at constant volume
    - $C_V = \wrap{\pder{Q}{T}}{V} = \wrap{\frac{TdS}{dT}}{V} = T\wrap{\pder{S}{T}}{V}$
    - Alternatively: $C_V = \wrap{\pder{dE+pdV}{T}}{V} = \wrap{\pder{E}{T}}{V}$
    - Molar specific heat: $c_V = \frac{C_V}{n}$
  - heat capacity at constant pressure
    - $C_p = \wrap{\frac{dQ}{dT}}{p} = T\wrap{\pder{S}{T}}{p}$
    - Alternatively:
  - $C_p - C_V = VT \frac{\alpha^2}{\kappa}$ where:
    - $\alpha\equiv \frac{1}{V}\wrap{\pder{V}{T}}{p}$ is the Volume coefficient of Expansion
    - $\kappa\equiv -\frac{1}{V}\wrap{\pder{V}{p}}{T}$ is Isothermal compressibility
 - Determine homogeneous substance undergoes a state change from macroscopic state A to macroscopic state B
  - $\Delta S=S(T,V) - S(T_0, V_0)$
  - $\Delta E=E(T,V) - E(T_0, V_0)$

#### Show stuff

Starting with First Law:
$$\begin{aligned}
dQ = TdS &= TdS(T,p) \\
 &= T \wrap{\wrap{\pder{S}{T}}{p} dT + \wrap{\pder{S}{p}}{T} dp}}{} \\
 &= C_p dT + T \wrap{\pder{S}{p} }{T} dp
\end{aligned}$$

Now let us expand the total differential of pressure:

$$\begin{aligned}
&= C_p dT + T \wrap{\pder{S}{p} }{T} \wrap{ \wrap{\pder{p}{V}}{T} dV + \wrap{\pder{p}{T}}{V} dT }{} \\
dQ &= \wrap{C_p + T \wrap{\pder{S}{p} }{T} \wrap{\pder{p}{T}}{V} }{} dT + T \wrap{\pder{S}{p} }{T}\wrap{\pder{p}{V}}{T} dV
\end{aligned}$$

Now we can Calculate the change in heat at fixed volume: $dV = 0$

$$\begin{aligned}
dQ &= \wrap{ C_p + T \wrap{\pder{S}{p} }{T} \wrap{\pder{p}{T}}{V} }{}dT \\
\\
\wrap{\pder{Q}{T}}{V} &= C_p + T \wrap{\pder{S}{p} }{T} \wrap{\pder{p}{T}}{V} \\
\\
\wrap{\pder{Q}{T}}{V} & \text{ is really just the specific heat at constant volume} \\
\\
C_V &= C_p + T \wrap{\pder{S}{p} }{T} \wrap{\pder{p}{T}}{V} \\
\\
C_p - C_V &= -T \wrap{\pder{p}{T}}{V}\wrap{\pder{S}{p} }{T}
\end{aligned}$$

?> Recall with Maxwell:
?> $$\wrap{\pder{S}{p}}{T} = -\wrap{\pder{V}{T}}{p} $$

$$\begin{aligned}
C_p - C_V &= -T \wrap{\pder{p}{T}}{V}\wrap{-\pder{V}{T}}{p} \\
&= T \wrap{\pder{p}{T}}{V}\wrap{\pder{V}{T}}{p}
\end{aligned}$$

?> Recall the coefficients we introduced at the start of class:
?> $$\alpha\equiv \frac{1}{V}\wrap{\pder{V}{T}}{p}$$ and $$\kappa\equiv -\frac{1}{V}\wrap{\pder{V}{p}}{T}$$

Text

$$\begin{aligned}
C_p - C_V &= T \wrap{\pder{p}{T}}{V}\wrap{\pder{V}{T}}{p} \\
  &= T \wrap{ \frac{\wrap{\pder{V}{T}}{p}} {\wrap{\pder{V}{p}}{T}}}{} \wrap{V\alpha}{p} \\
  &= T \wrap{ \frac{-V\alpha}{-V\kappa} \frac{V\alpha}{p} }{} \\
  C_p - C_V &= TV \frac{\alpha^2}{\kappa}
\end{aligned}$$

$$\begin{aligned}
c_p &= 3
\end{aligned}$$

Text

#### SWBQ

Use the following relationship to show that for an ideal gas $C_p - C_V = nR$:

$$C_p - C_V = TV \frac{\alpha^2}{\kappa}$$

Work:

$$\begin{aligned}
\alpha & \equiv \frac{1}{V}\wrap{\pder{V}{T}}{p} \\
  &= \frac{1}{V}\wrap{\frac{nR}{p}}{} \\
  &= \frac{nR}{Vp}
\end{aligned}$$

V = {nRT}{p}

$$\begin{aligned}
\kappa & \equiv -\frac{1}{V}\wrap{\pder{V}{p}}{T} \\
  &= -\frac{-nRT}{V p^2}
\end{aligned}$$

$$\begin{aligned}
C_p - C_V &= TV \frac{\alpha^2}{\kappa} \\
&= TV \frac{\wrap{\frac{nR}{Vp}}^2 {}}{-\frac{-nRT}{V p^2}} \\
&= nR TV \frac{nR}{V^2 p^2}\frac{V p^2}{nRT} \\
&= nR
\end{aligned}$$
